Added large part of proof to show that removing scoped variable declarations preserves the semantics.
Added separate file for subset conditions on AST.

Still open:
* Under certain conditions can move quantifier in a postcondition in front
of the weakest precondition
* Need to prove that all the new names concatenated have no duplicates
(in order to invoke the main lemma regarding removal of scoped variables)

RemoveScopedVarsProof.dfy
@@ -1,10 +1,13 @@
 include "BoogieSemantics.dfy"
 include "DesugarScopedVarsImpl.dfy"
+include "MakeScopedVarsUniqueProof.dfy"
 include "Naming.dfy"
+include "ForallAppend.dfy"
 include "dafny-libraries/src/Collections/Sequences/Seq.dfy"
 include "dafny-libraries/src/Collections/Maps/Maps.dfy"
+include "AstSubsetPredicates.dfy"
 
-module MakeScopedVarsUniqueProof {
+module RemoveScopedVarsUniqueProof {
 
   import opened BoogieLang
   import opened BoogieSemantics
@@ -13,13 +16,20 @@ module MakeScopedVarsUniqueProof {
   import Util
   import opened Wrappers
   import opened DesugarScopedVarsImpl
+  import MakeScopedVarsUniqueProof
   import opened Naming
+  import ForallAppend
+  import opened AstSubsetPredicates
 
-  //predicate StatesAgreeOnSet<A(!new)>(s1: state<A>, s2: state<A>, 
-  predicate PredDepend<A(!new)>(p: Predicate<A>, depVars: set<var_name>)
+  predicate {:opaque} StateEqualOn<A(!new)>(s1: state<A>, s2: state<A>, xs: set<var_name>)
+  {
+    forall x | x in xs :: Maps.Get(s1, x) == Maps.Get(s2, x)
+  }
+
+  predicate {:opaque} PredDepend<A(!new)>(p: Predicate<A>, depVars: set<var_name>)
   {
     forall s1, s2 | 
-      (forall x | x in depVars :: Maps.Get(s1, x) == Maps.Get(s2, x)) :: 
+      StateEqualOn(s1, s2, depVars) :: 
       p(s1) == p(s2)
   }
 
@@ -30,8 +40,22 @@ module MakeScopedVarsUniqueProof {
     && (forall lbl | lbl in post.scopes.Keys :: PredDepend(post.scopes[lbl], depVars))
   }
 
+  lemma {:verify false} PredDependMonotone<A(!new)>(p: Predicate<A>, depVars: set<var_name>, depVars': set<var_name>)
+  requires depVars <= depVars'
+  requires PredDepend(p, depVars)
+  ensures PredDepend(p, depVars')
+  { }
+
+  lemma {:verify false} PostDependMonotone<A(!new)>(post: WpPost<A>, depVars: set<var_name>, depVars': set<var_name>)
+  requires depVars <= depVars'
+  requires PostDepend(post, depVars)
+  ensures PostDepend(post, depVars')
+  { }
+
   lemma {:verify false} RemoveScopedVarsPreserveWf(c: Cmd, activeVars: set<var_name>)
-    requires c.WellFormedVars(activeVars)
+    requires 
+     && c.WellFormedVars(activeVars)
+     && NoLoopsNoIfCond(c)
     ensures 
       var (c', decls) := RemoveScopedVars(c);
       c'.WellFormedVars(activeVars+GetVarNames(decls))
@@ -80,34 +104,611 @@ module MakeScopedVarsUniqueProof {
 
       CmdWellFormedVarsLarger(c1', activeVars+GetVarNames(decls1), activeVars+GetVarNames(decls));
       CmdWellFormedVarsLarger(c2', activeVars+GetVarNames(decls2), activeVars+GetVarNames(decls));
-    case _ => assume false;
   }
 
-  lemma RemoveScopedVarsCorrect<A(!new)>(a: absval_interp<A>, activeVars: set<var_name>, c: Cmd, post: WpPost<A>)
+
+  lemma {:verify true} WpSimplePredDepend<A(!new)>(a: absval_interp<A>, xs: set<var_name>, sc: SimpleCmd, p: Predicate<A>)
+    requires sc.WellFormedVars(xs)
+    requires PredDepend(p, xs)
+    ensures PredDepend(WpSimpleCmd(a, sc, p), xs)
+  {
+    reveal PredDepend();
+    forall s1, s2 | StateEqualOn(s1, s2, xs)
+    ensures WpSimpleCmd(a, sc, p)(s1) == WpSimpleCmd(a, sc, p)(s2)
+    {
+      reveal StateEqualOn();
+      match sc
+      case Skip =>
+      case Assert(e) =>
+        assert EvalExpr(a, e, s1) == EvalExpr(a, e, s2) by {
+          EvalExprFreeVarEq(a, e, s1, s2);
+        }
+      case Assume(e) =>
+        assert EvalExpr(a, e, s1) == EvalExpr(a, e, s2) by {
+          EvalExprFreeVarEq(a, e, s1, s2);
+        }
+      case Assign(x, t, e) =>
+        assert EvalExpr(a, e, s1) == EvalExpr(a, e, s2) by {
+          EvalExprFreeVarEq(a, e, s1, s2);
+        }
+      case Havoc(varDecls) => 
+        ForallPredDepend(a, xs, varDecls, p);
+      case SeqSimple(sc1, sc2) => 
+        calc {
+          WpSimpleCmd(a, SeqSimple(sc1, sc2), p)(s1);
+          WpSimpleCmd(a, sc1, WpSimpleCmd(a, sc2, p))(s1);
+          { assert PredDepend(WpSimpleCmd(a, sc2, p), xs) by {
+              WpSimplePredDepend(a, xs, sc2, p);
+            }
+            WpSimplePredDepend(a, xs, sc1, WpSimpleCmd(a, sc2, p));
+          }
+          WpSimpleCmd(a, sc1, WpSimpleCmd(a, sc2, p))(s2);
+        }
+    }
+  }
+
+  lemma ResetVarsStateAux1<A(!new)>(s1: state<A>, s2: state<A>, xs: set<var_name>, d: seq<VarDecl>, s: state<A>, s': state<A>)
+  requires StateEqualOn(s1, s2, xs)
+  requires StateEqualOn(s, s', xs)
+  ensures StateEqualOn(ResetVarsState(d, s, s1), ResetVarsState(d, s', s2), xs)
+  {
+    reveal StateEqualOn();
+    if |d| > 0 {
+      var x := d[0].0;
+      var s1' := ResetVarsState(d[1..], s, s1);
+      var s2' := ResetVarsState(d[1..], s', s2);
+      assert StateEqualOn(s1', s2', xs);
+    }
+  }
+
+  lemma ResetVarsStateAux2<A(!new)>(s: state<A>, sOrig: state<A>, xs: set<var_name>, d: seq<VarDecl>)
+  requires GetVarNames(d) !! xs
+  ensures StateEqualOn(s, ResetVarsState(d, s, sOrig), xs)
+  {
+    reveal StateEqualOn();
+  }
+
+  lemma ResetVarsPredAux1<A(!new)>(s1: state<A>, s2: state<A>, xs: set<var_name>, d: seq<VarDecl>, p: Predicate<A>, s: state<A>, s': state<A>)
+  requires PredDepend(p, xs)
+  requires StateEqualOn(s1, s2, xs)
+  requires StateEqualOn(s, s', xs)
+  ensures ResetVarsPred(d, p, s1)(s) == ResetVarsPred(d, p, s2)(s')
+  {
+    reveal PredDepend();
+
+    assert StateEqualOn(s, s', xs);
+    if |d| > 0 {
+
+      assert ResetVarsPred(d, p, s1)(s) == ResetVarsPred(d, p, s2)(s') by {
+        calc {
+          ResetVarsPred(d, p, s1)(s);
+          p(ResetVarsState(d, s, s1));
+          { assert StateEqualOn(ResetVarsState(d, s, s1), ResetVarsState(d, s', s2), xs) by {
+              ResetVarsStateAux1(s1, s2, xs, d, s, s');
+            } 
+          }
+          p(ResetVarsState(d, s', s2));
+          ResetVarsPred(d, p, s2)(s');
+        }
+      }
+    }
+ }
+
+  lemma ResetVarsPredAux1'<A(!new)>(s1: state<A>, s2: state<A>, xs: set<var_name>, d: seq<VarDecl>, p: Predicate<A>)
+  requires PredDepend(p, xs)
+  requires StateEqualOn(s1, s2, xs)
+  ensures forall s: state<A> :: ResetVarsPred(d, p, s1)(s) == ResetVarsPred(d, p, s2)(s)
+  {
+    reveal StateEqualOn();
+    forall s: state<A> | true
+    { 
+      ResetVarsPredAux1(s1, s2, xs, d, p, s, s);
+    }
+  }
+
+  lemma ResetVarsPredAux2<A(!new)>(s: state<A>, xs: set<var_name>, d: seq<VarDecl>, p: Predicate<A>)
+  requires PredDepend(p, xs)
+  ensures PredDepend(ResetVarsPred(d, p, s), xs)
+  {
+    reveal StateEqualOn();
+    forall s1, s2 | StateEqualOn(s1, s2, xs)
+    ensures ResetVarsPred(d, p, s)(s1) == ResetVarsPred(d, p, s)(s2)
+    {
+      ResetVarsPredAux1(s, s, xs, d, p, s1, s2);
+    }
+    reveal PredDepend();
+  }
+
+  lemma ResetVarsPredAux3<A(!new)>(s: state<A>, xs: set<var_name>, d: seq<VarDecl>, p: Predicate<A>)
+  requires PredDepend(p, xs)
+  requires GetVarNames(d) !! xs
+  ensures forall s' :: ResetVarsPred(d, p, s)(s') == p(s')
+  {
+    forall s' | true
+    ensures ResetVarsPred(d, p, s)(s') == p(s')
+    {
+      calc {
+        ResetVarsPred(d, p, s)(s');
+        p(ResetVarsState(d, s', s));
+        { 
+          assert StateEqualOn(s', ResetVarsState(d, s', s), xs) by {
+            ResetVarsStateAux2(s', s, xs, d);
+          } 
+          reveal PredDepend();
+        }
+        p(s');
+      }
+    }
+  }
+
+  lemma ResetVarsPostAux1<A(!new)>(s1: state<A>, s2: state<A>, xs: set<var_name>, d: seq<VarDecl>, post: WpPost<A>)
+  requires PostDepend(post, xs)
+  requires StateEqualOn(s1, s2, xs)
+  ensures PostPointwise(ResetVarsPost(d, post, s1), ResetVarsPost(d, post, s2))
+  {
+    ResetVarsPredAux1'(s1, s2, xs, d, post.normal);
+    ResetVarsPredAux1'(s1, s2, xs, d, post.currentScope);
+    forall l | l in post.scopes.Keys
+    ensures forall s :: ResetVarsPred(d, post.scopes[l], s1)(s) == ResetVarsPred(d, post.scopes[l], s2)(s)
+    { ResetVarsPredAux1'(s1, s2, xs, d, post.scopes[l]); }
+  }
+
+  lemma ResetVarsPostAux2<A(!new)>(s: state<A>, xs: set<var_name>, d: seq<VarDecl>, post: WpPost<A>)
+  requires PostDepend(post, xs)
+  ensures PostDepend(ResetVarsPost(d, post, s), xs)
+  {
+    ResetVarsPredAux2(s, xs, d, post.normal);
+    ResetVarsPredAux2(s, xs, d, post.currentScope);
+    forall l | l in post.scopes.Keys
+    ensures PredDepend(ResetVarsPred(d, post.scopes[l], s), xs)
+    { ResetVarsPredAux2(s, xs, d, post.scopes[l]); }
+  }
+
+  lemma ResetVarsPostAux3<A(!new)>(s: state<A>, xs: set<var_name>, d: seq<VarDecl>, post: WpPost<A>)
+  requires PostDepend(post, xs)
+  requires GetVarNames(d) !! xs
+  ensures PostPointwise(ResetVarsPost(d, post, s), post)
+  {
+    ResetVarsPredAux3(s, xs, d, post.normal);
+    ResetVarsPredAux3(s, xs, d, post.currentScope);
+    forall l | l in post.scopes.Keys
+    ensures forall s' :: ResetVarsPred(d, post.scopes[l], s)(s') == post.scopes[l](s')
+    { ResetVarsPredAux3(s, xs, d, post.scopes[l]); }
+  }
+
+  lemma {:verify false} WpPredDepend<A(!new)>(a: absval_interp<A>, xs: set<var_name>, c: Cmd, post: WpPost<A>)
+    requires c.WellFormedVars(xs)
+    requires NoLoopsNoIfCond(c)
+    requires LabelsWellDefAux(c, post.scopes.Keys)
+    requires PostDepend(post, xs)
+    ensures PredDepend(WpCmd(a, c, post), xs)
+    decreases c
+  {
+    match c
+    case SimpleCmd(sc) => reveal WpCmd(); WpSimplePredDepend(a, xs, sc, post.normal);
+    case Break(_) => reveal WpCmd();
+    case Scope(optLabel, varDecls, body) => 
+      var updatedScopes := 
+        if optLabel.Some? then 
+          post.scopes[optLabel.value := post.normal]
+        else post.scopes;
+
+      assert updatedScopes.Keys == if optLabel.Some? then {optLabel.value} + post.scopes.Keys else post.scopes.Keys;
+      var post' := WpPost(post.normal, post.normal, updatedScopes);
+      
+      //s => ForallVarDecls( a, varDecls, WpCmd(a, body, ResetVarsPost(varDecls, post', s)) )(s)
+      forall s1, s2 : state<A> | StateEqualOn(s1, s2, xs)
+      ensures WpCmd(a, c, post)(s1) == WpCmd(a, c, post)(s2)
+      {
+        assert L1:
+          ForallVarDecls( a, varDecls, WpCmd(a, body, ResetVarsPost(varDecls, post', s1)) )(s1) 
+        == 
+          ForallVarDecls( a, varDecls, WpCmd(a, body, ResetVarsPost(varDecls, post', s2)) )(s1) by {
+            assert PostPointwise(ResetVarsPost(varDecls, post', s1), ResetVarsPost(varDecls, post', s2)) by {
+              ResetVarsPostAux1(s1, s2, xs, varDecls, post');
+            }
+
+            WpCmdPointwise2(a, body, ResetVarsPost(varDecls, post', s1), ResetVarsPost(varDecls, post', s2));
+
+            ForallVarDeclsPointwise( 
+              a, 
+              varDecls, 
+              WpCmd(a, body, ResetVarsPost(varDecls, post', s1)), 
+              WpCmd(a, body, ResetVarsPost(varDecls, post', s2)),
+              s1);
+          }
+        
+        assert L2:
+          PredDepend(ForallVarDecls( a, varDecls, WpCmd(a, body, ResetVarsPost(varDecls, post', s2)) ), xs) by {
+          
+          assert PostDepend(ResetVarsPost(varDecls, post', s2), xs) by {
+            ResetVarsPostAux2(s2, xs, varDecls, post');
+          }
+
+          assert PostDepend(ResetVarsPost(varDecls, post', s2), xs+GetVarNames(varDecls)) by {
+            PostDependMonotone(ResetVarsPost(varDecls, post', s2), xs, xs+GetVarNames(varDecls));
+          }
+          
+          WpPredDepend(a, xs+GetVarNames(varDecls), body, ResetVarsPost(varDecls, post', s2));
+
+          ForallPredDepend(a, xs, varDecls, WpCmd(a, body, ResetVarsPost(varDecls, post', s2)));
+        }
+
+        calc {
+          WpCmd(a, c, post)(s1);
+          { reveal WpCmd(); }
+          ForallVarDecls( a, varDecls, WpCmd(a, body, ResetVarsPost(varDecls, post', s1)) )(s1);
+          { 
+            reveal L1;
+            reveal L2;
+            reveal PredDepend();
+          }
+          ForallVarDecls( a, varDecls, WpCmd(a, body, ResetVarsPost(varDecls, post', s2)) )(s2);
+          { reveal WpCmd(); }
+          WpCmd(a, c, post)(s2);
+        }
+      }
+      reveal PredDepend();
+    case If(None, thn, els) => 
+      reveal WpCmd();
+      forall s1,s2 | StateEqualOn(s1, s2, xs)
+      ensures WpCmd(a, c, post)(s1) == WpCmd(a, c, post)(s2)
+      {
+        calc {
+          WpCmd(a, If(None, thn, els), post)(s1);
+          Util.AndOpt(WpCmd(a, thn, post)(s1), WpCmd(a, els, post)(s1));
+          { WpPredDepend(a, xs, thn, post); 
+            WpPredDepend(a, xs, els, post);
+            reveal PredDepend(); }
+          Util.AndOpt(WpCmd(a, thn, post)(s2), WpCmd(a, els, post)(s2));
+        }
+      }
+      reveal PredDepend();
+    case Seq(c1, c2) => 
+      reveal WpCmd();
+      reveal PredDepend();
+  }
+
+  lemma {:verify false} StateUpdVarDeclsEqOutsideDecls<A>(s: state<A>, decls: seq<VarDecl>, vs: seq<Val<A>>, x: var_name)
+    requires |decls| == |vs|
+    requires x !in GetVarNames(decls)
+    ensures Maps.Get(StateUpdVarDecls(s, decls, vs), x) == Maps.Get(s, x)
+  { }
+
+  lemma {:verify false} StateUpdVarDeclsEqOnDecls<A>(s1: state<A>, s2: state<A>, decls: seq<VarDecl>, vs: seq<Val<A>>, x: var_name)
+    requires |decls| == |vs|
+    requires x in GetVarNames(decls)
+    ensures  Maps.Get(StateUpdVarDecls(s1, decls, vs), x) == Maps.Get(StateUpdVarDecls(s2, decls, vs), x)
+  {
+    if |decls| > 0 {
+      var y := decls[0].0;
+
+      if x != y {
+        var s1' := StateUpdVarDecls(s1, decls[1..], vs[1..]);
+        var s2' := StateUpdVarDecls(s2, decls[1..], vs[1..]);
+
+        assert Maps.Get(s1', x) == Maps.Get(s2', x) by {
+          StateUpdVarDeclsEqOnDecls(s1, s2, decls[1..], vs[1..], x);
+        }
+      }
+    }
+  }
+
+  lemma {:verify false} ForallPredDepend<A(!new)>(a: absval_interp<A>, activeVars: set<var_name>, decls: seq<VarDecl>, p: Predicate<A>)
+    requires PredDepend(p, activeVars+GetVarNames(decls))
+    ensures PredDepend(ForallVarDecls(a, decls, p), activeVars)
+  {
+    if |decls| == 0 {
+      reveal ForallVarDecls();
+    } else {
+      forall s1,s2: state<A> | (forall x | x in activeVars :: Maps.Get(s1, x) == Maps.Get(s2, x))
+      ensures ForallVarDecls(a, decls, p)(s1) == ForallVarDecls(a, decls, p)(s2)
+      {
+         forall vs | ValuesRespectDecls(a, vs, decls)
+         ensures p(StateUpdVarDecls(s1, decls, vs)) == p(StateUpdVarDecls(s2, decls, vs))
+         {
+           var s1' := StateUpdVarDecls(s1, decls, vs);
+           var s2' := StateUpdVarDecls(s2, decls, vs);
+
+           forall x | x in activeVars + GetVarNames(decls) 
+           ensures Maps.Get(s1', x) == Maps.Get(s2', x)
+           {
+            if x in GetVarNames(decls) {
+              StateUpdVarDeclsEqOnDecls(s1, s2, decls, vs, x);
+            } else {
+              assert x in activeVars && x !in GetVarNames(decls);
+              StateUpdVarDeclsEqOutsideDecls(s1, decls, vs, x);
+              StateUpdVarDeclsEqOutsideDecls(s2, decls, vs, x);
+            }
+           }
+         }
+
+         ForallVarDeclsEquiv(a, decls, decls, p, p, s1, s2);
+      }
+    }
+  }
+
+  lemma {:verify false} ForallWpPredDepend<A(!new)>(a: absval_interp<A>, activeVars: set<var_name>, decls: seq<VarDecl>, c: Cmd, post: WpPost<A>)
+    requires c.WellFormedVars(activeVars+GetVarNames(decls))
+    requires LabelsWellDefAux(c, post.scopes.Keys)
+    requires PostDepend(post, activeVars)
+    ensures PredDepend(ForallVarDecls(a, decls, WpCmd(a, c, post)), activeVars)
+  {
+    assert PredDepend(WpCmd(a, c, post), activeVars+GetVarNames(decls)) by {
+      assert PostDepend(post, activeVars+GetVarNames(decls)) by {
+        PostDependMonotone(post, activeVars, activeVars+GetVarNames(decls));
+      }
+      WpPredDepend(a, activeVars+GetVarNames(decls), c, post);
+    }
+
+    ForallPredDepend(a, activeVars, decls, WpCmd(a, c, post));
+  }
+
+  lemma PullForallWpSimpleCmd<A(!new)>(a: absval_interp<A>, xs: set<var_name>, cxs: set<var_name>, d: seq<VarDecl>, sc: SimpleCmd, p: Predicate<A>, s: state<A>)
+    requires xs !! GetVarNames(d)
+   // requires PredDepend(p, xs+GetVarNames(d))
+    requires && sc.WellFormedVars(xs+cxs) /** needed to make sure that sc and d do not intefere */
+             && cxs !! GetVarNames(d)
+    ensures 
+      WpSimpleCmd(a, sc, ForallVarDecls(a, d, p))(s)
+    ==
+      ForallVarDecls(a, d, WpSimpleCmd(a, sc, p))(s)
+  { assume false; }
+  /*
+  {
+    match sc 
+    case Skip =>
+    case Assert(e) => 
+      /* EvalExprFreeVarEq(a, e, s1, s2); */
+      assume false;
+    case Assume(e) => 
+      /*
+        var eEval := ExprEvalBoolOpt(a, e, s); 
+        if eEval == None then
+          None
+        else if eEval == Some(false) then
+          Some(true)
+        else 
+          var postEval :- post(s); 
+          Some(postEval)
+      */
+      var eEval := ExprEvalBoolOpt(a, e, s); 
+      assume false;
+    case Assign(x, t, e) => assume false;
+    case Havoc(varDecls) => assume false;
+    case SeqSimple(sc1, sc2) => assume false;
+  }
+  */
+
+  lemma PullForallWp<A(!new)>(a: absval_interp<A>, xs: set<var_name>, cxs: set<var_name>, d: seq<VarDecl>, c: Cmd, p: Predicate<A>, post: WpPost<A>, s: state<A>)
+    requires LabelsWellDefAux(c, post.scopes.Keys)
+    requires && PostDepend(post, xs) /** needed to make sure that d is not captured in post */
+             && xs !! GetVarNames(d)
+   // requires PredDepend(p, xs+GetVarNames(d))
+    requires && c.WellFormedVars(xs+cxs) /** needed to make sure that c and d do not intefere */
+             && cxs !! GetVarNames(d)
+    ensures 
+      WpCmd(a, c, WpPost(ForallVarDecls(a, d, p), post.currentScope, post.scopes))(s)
+    ==
+      ForallVarDecls(a, d, WpCmd(a, c, WpPost(p, post.currentScope, post.scopes)))(s)
+
+
+  lemma HasNoDuplicatesAppend<T>(s1: seq<T>, s2: seq<T>)
+  requires Sequences.HasNoDuplicates(s1+s2)
+  ensures 
+    && Sequences.HasNoDuplicates(s1)
+    && Sequences.HasNoDuplicates(s2)
+  {
+    reveal Sequences.HasNoDuplicates();
+    forall i, j | 0 <= i < |s1| && 0 <= j < |s1| && i != j 
+    ensures s1[i] != s1[j]
+    {
+      assert s1[i] == (s1+s2)[i];
+      assert s1[j] == (s1+s2)[j];
+    }
+
+    forall i, j | 0 <= i < |s2| && 0 <= j < |s2| && i != j 
+    ensures s2[i] != s2[j]
+    {
+      assert s2[i] == (s1+s2)[|s1|+i];
+      assert s2[j] == (s1+s2)[|s1|+j];
+    }
+  }
+
+  lemma HasNoDuplicatesAppDisj(s1: seq<VarDecl>, s2: seq<VarDecl>)
+  requires Sequences.HasNoDuplicates(GetVarNamesSeq(s1+s2))
+  ensures GetVarNames(s1) !! GetVarNames(s2)
+  {
+    var s12 := GetVarNamesSeq(s1+s2);
+    
+    forall x | x in GetVarNames(s1)
+    ensures x !in GetVarNames(s2)
+    {
+      var i :| 0 <= i < |s1| && s1[i].0 == x;
+      assert s12[i] == x;
+
+      forall j | 0 <= j < |s2|
+      ensures x != s2[j].0
+      {
+        assert s12[|s1|+j] == s2[j].0;
+        reveal Sequences.HasNoDuplicates();
+      }
+    }
+  }
+
+  lemma RemoveScopedVarsGetDecls(c: Cmd)
+    requires NoLoopsNoIfCond(c)
+    ensures
+      var (c', decls) := RemoveScopedVars(c);
+      GetDecls(c) == decls
+  { }
+ 
+  lemma {:verify true} RemoveScopedVarsCorrect<A(!new)>(a: absval_interp<A>, activeVars: set<var_name>, c: Cmd, post: WpPost<A>)
     requires 
       var (c', decls) := RemoveScopedVars(c);
       && LabelsWellDefAux(c, post.scopes.Keys) 
       && LabelsWellDefAux(c', post.scopes.Keys) 
       && c.WellFormedVars(activeVars) 
       && PostDepend(post, activeVars)
+      && Sequences.HasNoDuplicates(GetVarNamesSeq(GetDecls(c)))
+      && NoLoopsNoIfCond(c)
       && activeVars !! GetVarNames(decls)
     ensures 
       var (c', decls) := RemoveScopedVars(c);
-      forall s :: WpCmd(a, c, post)(s) == ForallVarDecls(a, decls, WpCmd(a, c', post))(s)
+      (forall s :: WpCmd(a, c, post)(s) == ForallVarDecls(a, decls, WpCmd(a, c', post))(s))
+    decreases c
     {
       var (c', decls) := RemoveScopedVars(c);
-      assert c'.WellFormedVars(activeVars+GetVarNames(decls)) by {
-        RemoveScopedVarsPreserveWf(c, activeVars);
+      assert GetDecls(c) == decls by {
+        RemoveScopedVarsGetDecls(c);
       }
 
       forall s | true
-      ensures WpCmd(a, c, post)(s) == ForallVarDecls(a, decls, WpCmd(a, c', post))(s)
+      ensures 
+        WpCmd(a, c, post)(s) == ForallVarDecls(a, decls, WpCmd(a, c', post))(s)
       {
         match c 
         case SimpleCmd(sc) => ForallVarDeclsEmpty(a, WpCmd(a, c', post)); 
         case Break(_) => ForallVarDeclsEmpty(a, WpCmd(a, c', post)); 
-        case Scope(_, varDecls, body) => assume false;
-        case If(None, thn, els) => assume false;
+        case Scope(optLabel, varDecls, body) => 
+
+          var (body', declsBody) := RemoveScopedVars(body);
+
+          var updatedScopes := 
+            if optLabel.Some? then 
+              post.scopes[optLabel.value := post.normal]
+            else post.scopes;
+
+          assert updatedScopes.Keys == if optLabel.Some? then {optLabel.value} + post.scopes.Keys else post.scopes.Keys;
+          var post' := WpPost(post.normal, post.normal, updatedScopes);
+
+          assert GetVarNames(varDecls) !! GetVarNames(declsBody) by {
+            HasNoDuplicatesAppDisj(varDecls, declsBody);
+          }
+
+          calc {
+            WpCmd(a, c, post)(s);
+            { reveal WpCmd(); }
+            ForallVarDecls( a, varDecls, WpCmd(a, body, ResetVarsPost(varDecls, post', s)) )(s);
+            { 
+              ResetVarsPostAux3(s, activeVars, varDecls, post'); 
+              WpCmdPointwise2(a, body, ResetVarsPost(varDecls, post', s), post');
+              ForallVarDeclsPointwise(a, varDecls, WpCmd(a, body, ResetVarsPost(varDecls, post', s)), WpCmd(a, body, post'), s);
+            }
+            ForallVarDecls( a, varDecls, WpCmd(a, body, post') )(s);
+            { 
+              assert PostDepend(post', activeVars+GetVarNames(varDecls)) by {
+                PostDependMonotone(post', activeVars, activeVars+GetVarNames(varDecls));
+              }
+              assert Sequences.HasNoDuplicates(GetVarNamesSeq(varDecls + declsBody));
+              assert Sequences.HasNoDuplicates(GetVarNamesSeq(declsBody)) by {
+                assert GetVarNamesSeq(varDecls+declsBody) == GetVarNamesSeq(varDecls)+GetVarNamesSeq(declsBody);
+                HasNoDuplicatesAppend(GetVarNamesSeq(varDecls), GetVarNamesSeq(declsBody));
+              }
+              assert declsBody == GetDecls(body) by {
+                RemoveScopedVarsGetDecls(body);
+              }
+
+              RemoveScopedVarsCorrect(a, activeVars+GetVarNames(varDecls), body, post'); 
+              ForallVarDeclsPointwise(a, varDecls, WpCmd(a, body, post'), ForallVarDecls(a, declsBody, WpCmd(a, body', post')), s);
+            }
+            ForallVarDecls( a, varDecls, ForallVarDecls(a, declsBody, WpCmd(a, body', post') ))(s);
+            { ForallAppend.ForallVarDeclsAppend(a, varDecls, declsBody, WpCmd(a, body', post'), s); }
+            ForallVarDecls( a, varDecls+declsBody, WpCmd(a, body', post') )(s);
+            { assert ResetVarsPost([], post', s) == post'; }
+            ForallVarDecls( a, varDecls+declsBody, WpCmd(a, body', ResetVarsPost([], post', s)) )(s);
+            { reveal ForallVarDecls(); }
+            ForallVarDecls( a, varDecls+declsBody, ForallVarDecls(a, [], WpCmd(a, body', ResetVarsPost([], post', s))) )(s);
+            { 
+              forall s' | true
+              ensures 
+                ForallVarDecls(a, [], WpCmd(a, body', ResetVarsPost([], post', s)))(s') ==
+                WpCmd(a, Scope(optLabel, [], body'), post)(s')
+              {
+                calc {
+                ForallVarDecls(a, [], WpCmd(a, body', ResetVarsPost([], post', s)))(s');
+                { 
+                  calc {
+                    ResetVarsPost([], post', s);
+                    post';
+                    ResetVarsPost([], post', s');
+                 }
+                }
+                ForallVarDecls(a, [], WpCmd(a, body', ResetVarsPost([], post', s')))(s');
+                }
+                reveal WpCmd();
+              }
+
+              ForallVarDeclsPointwise(
+                a, 
+                varDecls+declsBody, 
+                ForallVarDecls(a, [], WpCmd(a, body', ResetVarsPost([], post', s))), 
+                WpCmd(a, Scope(optLabel, [], body'), post), 
+                s); 
+            }
+            ForallVarDecls( a, varDecls+declsBody, WpCmd(a, Scope(optLabel, [], body'), post) )(s);
+          }
+        case If(None, thn, els) => 
+          var (thn', declsThn) := RemoveScopedVars(thn);
+          var (els', declsEls) := RemoveScopedVars(els);
+
+          assert 
+            && Sequences.HasNoDuplicates(GetVarNamesSeq(GetDecls(thn))) 
+            && Sequences.HasNoDuplicates(GetVarNamesSeq(GetDecls(els))) by {
+            assert GetVarNamesSeq(GetDecls(thn)+GetDecls(els)) == GetVarNamesSeq(GetDecls(thn)) + GetVarNamesSeq(GetDecls(els));
+            HasNoDuplicatesAppend(GetVarNamesSeq(GetDecls(thn)), GetVarNamesSeq(GetDecls(els)));
+          }
+
+          assert GetVarNames(declsThn) !! GetVarNames(declsEls) by {
+            HasNoDuplicatesAppDisj(declsThn, declsEls);
+          }
+
+          calc {
+            WpCmd(a, c, post)(s);
+            { reveal WpCmd(); }
+            Util.AndOpt(
+              WpCmd(a, thn, post)(s), 
+              WpCmd(a, els, post)(s)
+            );
+            { 
+              RemoveScopedVarsCorrect(a, activeVars, thn, post); 
+              RemoveScopedVarsCorrect(a, activeVars, els, post);
+            }
+            Util.AndOpt(
+              ForallVarDecls(a, declsThn, WpCmd(a, thn', post))(s),
+              ForallVarDecls(a, declsEls, WpCmd(a, els', post))(s)
+            );
+          }
+
+          calc {
+            ForallVarDecls(a, declsThn, WpCmd(a, thn', post))(s);
+            { assume false; }
+            ForallVarDecls(a, declsThn, ForallVarDecls(a, declsEls, WpCmd(a, thn', post)))(s);
+            { ForallAppend.ForallVarDeclsAppend(a, declsThn, declsEls, WpCmd(a, thn', post), s); }
+            ForallVarDecls(a, declsThn+declsEls, WpCmd(a, thn', post))(s);
+          }
+
+          calc {
+            ForallVarDecls(a, declsEls, WpCmd(a, els', post))(s);
+            { assume false; }
+            ForallVarDecls(a, declsThn, ForallVarDecls(a, declsEls, WpCmd(a, els', post)))(s);
+            { ForallAppend.ForallVarDeclsAppend(a, declsThn, declsEls, WpCmd(a, els', post), s); }
+            ForallVarDecls(a, declsThn+declsEls, WpCmd(a, els', post))(s);
+          }
+
+          var p' := s => Util.AndOpt(WpCmd(a, thn', post)(s), WpCmd(a, els', post)(s));
+          calc {
+            Util.AndOpt(
+              ForallVarDecls(a, declsThn+declsEls, WpCmd(a, thn', post))(s),
+              ForallVarDecls(a, declsThn+declsEls, WpCmd(a, els', post))(s)
+            );
+            { assume false; }
+            ForallVarDecls(a, declsThn+declsEls, p')(s);
+            { reveal WpCmd(); 
+              ForallVarDeclsPointwise(a, declsThn+declsEls, p', WpCmd(a, c', post), s);
+            }
+            ForallVarDecls(a, declsThn+declsEls, WpCmd(a, c', post))(s);
+          }
         case Seq(c1, c2) => 
           // WpPost(WpCmd(a, c2, post), post.currentScope, post.scopes)
           var (c1', decls1) := RemoveScopedVars(c1);
@@ -117,28 +718,74 @@ module MakeScopedVarsUniqueProof {
           var post2' := WpPost(ForallVarDecls(a, decls2, WpCmd(a, c2',post)), post.currentScope, post.scopes);
           var post2NoQuant' := WpPost(WpCmd(a, c2',post), post.currentScope, post.scopes);
 
+          assert c2'.WellFormedVars(activeVars+GetVarNames(decls2)) by {
+            RemoveScopedVarsPreserveWf(c2, activeVars);
+          }
+
+          assert GetVarNames(decls1) !! GetVarNames(decls2) by {
+            HasNoDuplicatesAppDisj(decls1, decls2);
+          }
+
           calc {
             WpCmd(a, Seq(c1, c2), post)(s);
             { reveal WpCmd(); }
             WpCmd(a, c1, post2)(s);
             { 
-              assert c2'.WellFormedVars(activeVars+GetVarNames(decls2)) by {
-                RemoveScopedVarsPreserveWf(c2, activeVars);
+              assert Sequences.HasNoDuplicates(GetVarNamesSeq(GetDecls(c2))) by {
+                assert GetVarNamesSeq(GetDecls(c1)+GetDecls(c2)) == GetVarNamesSeq(GetDecls(c1)) + GetVarNamesSeq(GetDecls(c2));
+                HasNoDuplicatesAppend(GetVarNamesSeq(GetDecls(c1)), GetVarNamesSeq(GetDecls(c2)));
               }
               RemoveScopedVarsCorrect(a, activeVars, c2, post); 
               WpCmdPointwise(a, c1, post2, post2', s);
             }
             WpCmd(a, c1, post2')(s);
-            { assume false; RemoveScopedVarsCorrect(a, activeVars, c1, post2'); }
+            { 
+              assert PredDepend(ForallVarDecls(a, decls2, WpCmd(a, c2',post)), activeVars) by {
+                ForallWpPredDepend(a, activeVars, decls2, c2', post);
+              }
+
+              assert Sequences.HasNoDuplicates(GetVarNamesSeq(GetDecls(c1))) by {
+                assert GetVarNamesSeq(GetDecls(c1)+GetDecls(c2)) == GetVarNamesSeq(GetDecls(c1)) + GetVarNamesSeq(GetDecls(c2));
+                HasNoDuplicatesAppend(GetVarNamesSeq(GetDecls(c1)), GetVarNamesSeq(GetDecls(c2)));
+              }
+              RemoveScopedVarsCorrect(a, activeVars, c1, post2'); 
+
+              //reveal due to opaque bug
+              reveal WpCmd();
+              reveal ForallVarDecls();
+            }
             ForallVarDecls(a, decls1, WpCmd(a, c1', post2'))(s);
-            { assume false; }
+            { 
+              //def. post2'
+            }
+            ForallVarDecls(a, decls1, WpCmd(a, c1', WpPost(ForallVarDecls(a, decls2, WpCmd(a, c2',post)), post.currentScope, post.scopes)))(s);
+            { 
+              forall s' | true
+              ensures 
+                WpCmd(a, c1', WpPost(ForallVarDecls(a, decls2, WpCmd(a, c2',post)), post.currentScope, post.scopes))(s') ==
+                ForallVarDecls(a, decls2, WpCmd(a, c1', post2NoQuant'))(s')
+              {
+                assert c1'.WellFormedVars(activeVars+GetVarNames(decls1)) by {
+                  RemoveScopedVarsPreserveWf(c1, activeVars);
+                }
+                PullForallWp(a, activeVars, GetVarNames(decls1), decls2, c1', WpCmd(a, c2',post), post, s');
+              }
+
+              ForallVarDeclsPointwise(a, decls1, WpCmd(a, c1', WpPost(ForallVarDecls(a, decls2, WpCmd(a, c2',post)), post.currentScope, post.scopes)),
+                                        ForallVarDecls(a, decls2, WpCmd(a, c1', post2NoQuant')), s);
+            }
             ForallVarDecls(a, decls1, ForallVarDecls(a, decls2, WpCmd(a, c1', post2NoQuant')))(s);
-            { assume false; }
+            { 
+              assert decls1 == GetDecls(c1) && decls2 == GetDecls(c2) by {
+                RemoveScopedVarsGetDecls(c1);
+                RemoveScopedVarsGetDecls(c2);
+              }
+              
+              ForallAppend.ForallVarDeclsAppend(a, decls1, decls2, WpCmd(a, c1', post2NoQuant'), s); }
             ForallVarDecls(a, decls1+decls2, WpCmd(a, c1', post2NoQuant'))(s);
-            { assume false; }
+            { reveal WpCmd(); }
             ForallVarDecls(a, decls1+decls2, WpCmd(a, Seq(c1', c2'), post))(s);
           }
-        case _ => assume false;
       }
 
       /* these reveal statements are needed due to a bug 
