ForallAppend.dfy
@@ -1,0 +1,317 @@
+include "BoogieSemantics.dfy"
+include "DesugarScopedVarsImpl.dfy"
+include "MakeScopedVarsUniqueProof.dfy"
+include "Naming.dfy"
+include "dafny-libraries/src/Collections/Sequences/Seq.dfy"
+include "dafny-libraries/src/Collections/Maps/Maps.dfy"
+
+module ForallAppend {
+
+  import opened BoogieLang
+  import opened BoogieSemantics
+  import Sequences = Seq
+  import Maps
+  import Util
+  import opened Wrappers
+  import opened DesugarScopedVarsImpl
+  import MakeScopedVarsUniqueProof
+  import opened Naming
+
+  lemma SeqSliceAux<A>(s1: seq<A>, s2: seq<A>)
+    requires |s1| > 0
+    ensures (s1+s2)[1..] == s1[1..]+s2
+  { }
+
+  //relies on Dafny checking pointwise equality when checking map equality
+  lemma StateUpdVarDeclsSwapAux<A(!new)>(s: state<A>, d: seq<VarDecl>, vs: seq<Val<A>>, x: var_name, v: Val<A>)
+  requires x !in GetVarNames(d)
+  requires |d| == |vs|
+  ensures StateUpdVarDecls(s, d, vs)[x := v] == StateUpdVarDecls(s[x := v], d, vs)
+  { }
+
+  lemma StateUpdVarDeclsSwap<A(!new)>(s: state<A>, d1: seq<VarDecl>, d2: seq<VarDecl>, vs1: seq<Val<A>>, vs2: seq<Val<A>>)
+    requires |d1| == |vs1| && |d2| == |vs2|
+    requires GetVarNames(d1) !! GetVarNames(d2)
+    ensures StateUpdVarDecls(StateUpdVarDecls(s, d1, vs1), d2, vs2) == StateUpdVarDecls(StateUpdVarDecls(s, d2, vs2), d1, vs1)
+  {
+    if |d1| > 0 {
+      var x := d1[0].0;
+      var v := vs1[0];
+      calc {
+        StateUpdVarDecls(StateUpdVarDecls(s, d2, vs2), d1, vs1);
+        StateUpdVarDecls(StateUpdVarDecls(s, d2, vs2), d1[1..], vs1[1..])[x := v];
+        { 
+          //induction hypothesis 
+        }
+        StateUpdVarDecls(StateUpdVarDecls(s, d1[1..], vs1[1..]), d2, vs2)[x := v];
+        { StateUpdVarDeclsSwapAux(StateUpdVarDecls(s, d1[1..], vs1[1..]), d2, vs2, x, v); }
+        StateUpdVarDecls(StateUpdVarDecls(s, d1[1..], vs1[1..])[x := v], d2, vs2);
+        StateUpdVarDecls(StateUpdVarDecls(s, d1, vs1), d2, vs2);
+      }
+    }
+  }
+
+  lemma StateUpdVarDeclsSplit<A(!new)>(s: state<A>, d1: seq<VarDecl>, d2: seq<VarDecl>, vs1: seq<Val<A>>, vs2: seq<Val<A>>)
+    requires |d1| == |vs1| && |d2| == |vs2|
+    ensures StateUpdVarDecls(s, d1+d2, vs1+vs2) == StateUpdVarDecls(StateUpdVarDecls(s, d2, vs2), d1, vs1)
+  {
+    if |d1| == 0 {
+      calc {
+        StateUpdVarDecls(s, d1+d2, vs1+vs2);
+        { 
+          assert d1+d2 == d2;
+          assert vs1+vs2 == vs2;
+        }
+        StateUpdVarDecls(s, d2, vs2);
+        StateUpdVarDecls(StateUpdVarDecls(s, d2, vs2), d1, vs1);
+      }
+    } else {
+      var x := d1[0].0;
+      var v := vs1[0];
+      assert (d1+d2)[0].0 == x;
+      assert (vs1+vs2)[0] == v;
+
+      var sA := StateUpdVarDecls(s, (d1+d2)[1..], (vs1+vs2)[1..]);
+      var sB := StateUpdVarDecls(StateUpdVarDecls(s, d2, vs2), d1[1..], vs1[1..]);
+
+      assert sA == sB by {
+        assert StateUpdVarDecls(s, d1[1..]+d2, vs1[1..]+vs2) == StateUpdVarDecls(StateUpdVarDecls(s, d2, vs2), d1[1..], vs1[1..]) by {
+          StateUpdVarDeclsSplit(s, d1[1..], d2, vs1[1..], vs2);
+        }
+        assert (d1+d2)[1..] == d1[1..]+d2 by {
+          SeqSliceAux(d1, d2); //DISCUSS (why can't Dafny prove the assertion without the helper lemma {:verify false}?)
+        }
+        assert (vs1+vs2)[1..] == vs1[1..]+vs2 by {
+          SeqSliceAux(vs1, vs2);
+        }
+      }
+
+      assert sA[x := v] == sB[x := v];
+
+      assert StateUpdVarDecls(s, d1+d2, vs1+vs2) == sA[x := v];
+      assert StateUpdVarDecls(StateUpdVarDecls(s, d2, vs2), d1, vs1) == sB[x := v];
+    }
+  }
+
+  lemma StateUpdVarDeclsSplit2<A(!new)>(s: state<A>, d1: seq<VarDecl>, d2: seq<VarDecl>, vs1: seq<Val<A>>, vs2: seq<Val<A>>)
+    requires |d1| == |vs1| && |d2| == |vs2|
+    requires GetVarNames(d1) !! GetVarNames(d2)
+    ensures StateUpdVarDecls(s, d1+d2, vs1+vs2) == StateUpdVarDecls(StateUpdVarDecls(s, d1, vs1), d2, vs2)
+  {
+    calc {
+      StateUpdVarDecls(s, d1+d2, vs1+vs2);
+      { StateUpdVarDeclsSplit(s, d1, d2, vs1, vs2); }
+      StateUpdVarDecls(StateUpdVarDecls(s, d2, vs2), d1, vs1);
+      { StateUpdVarDeclsSwap(s, d2, d1, vs2, vs1); }
+      StateUpdVarDecls(StateUpdVarDecls(s, d1, vs1), d2, vs2);
+    }
+  }
+
+  lemma ValuesRespectDeclsSlice<A(!new)>(a: absval_interp<A>, vs: seq<Val<A>>, varDecls: seq<VarDecl>, start: nat, end: nat)
+  requires ValuesRespectDecls(a, vs, varDecls)
+  requires 0 <= start <= end <= |varDecls|
+  ensures ValuesRespectDecls(a, vs[start..end], varDecls[start..end])
+  {
+    forall i | 0 <= i < |vs[start..end]|
+    ensures TypeOfVal(a, vs[start..end][i]) == varDecls[start..end][i].1 {
+      assert vs[start..end][i] == vs[start+i];
+      assert varDecls[start..end][i] == varDecls[start+i];
+      assert TypeOfValues(a, vs)[start+i] == seq(|varDecls|, i requires 0 <= i < |varDecls| => varDecls[i].1)[start+i];
+      assert TypeOfVal(a, vs[start+i]) == varDecls[start+i].1;
+    }
+  }
+
+  lemma ValuesRespectDeclsAppend<A(!new)>(
+    a: absval_interp<A>,
+    varDecls1: seq<(var_name, Ty)>, 
+    varDecls2: seq<(var_name, Ty)>, 
+    vs1: seq<Val<A>>,
+    vs2: seq<Val<A>>
+  )
+  requires ValuesRespectDecls(a, vs1, varDecls1)
+  requires ValuesRespectDecls(a, vs2, varDecls2)
+  ensures ValuesRespectDecls(a, vs1+vs2, varDecls1+varDecls2)
+  {
+    var vs := vs1+vs2;
+    var varDecls := varDecls1+varDecls2;
+    forall i | 0 <= i < |varDecls|
+    ensures TypeOfVal(a, vs[i]) == varDecls[i].1
+    {
+      if i < |vs1| {
+        assert vs[i] == vs1[i];
+        assert varDecls[i] == varDecls1[i];
+        assert TypeOfValues(a, vs1)[i] == seq(|varDecls|, i requires 0 <= i < |varDecls| => varDecls[i].1)[i];
+      } else {
+        var j := i-|vs1|;
+        assert vs[i] == vs2[j];
+        assert varDecls[i] == varDecls2[j];
+        assert TypeOfValues(a, vs2)[j] == seq(|varDecls2|, i requires 0 <= i < |varDecls2| => varDecls2[i].1)[j];
+      }
+    }
+  }
+ 
+  /** This proof has lots of duplication, there should be a way to make the 
+  proof shorter. */
+  lemma ForallVarDeclsAppend<A(!new)>(
+      a: absval_interp<A>, 
+      varDecls1: seq<(var_name, Ty)>, 
+      varDecls2: seq<(var_name, Ty)>, 
+      p: Predicate<A>,
+      s: state<A>)
+    requires GetVarNames(varDecls1) !! GetVarNames(varDecls2)
+    ensures    ForallVarDecls(a, varDecls1, ForallVarDecls(a, varDecls2, p))(s)
+            == ForallVarDecls(a, varDecls1+varDecls2, p)(s);
+    {
+      var varDecls := varDecls1+varDecls2;
+      if |varDecls1| == 0 {
+        calc {
+          ForallVarDecls(a, varDecls1, ForallVarDecls(a, varDecls2, p))(s);
+          { reveal ForallVarDecls(); }
+          ForallVarDecls(a, varDecls2, p)(s);
+          { assert varDecls2 == varDecls1+varDecls2; }
+          ForallVarDecls(a, varDecls1+varDecls2, p)(s);
+        }
+      } else if |varDecls2| == 0 {
+        calc {
+          ForallVarDecls(a, varDecls1, ForallVarDecls(a, varDecls2, p))(s);
+          { reveal ForallVarDecls(); }
+          ForallVarDecls(a, varDecls1, p)(s);
+          { assert varDecls1 == varDecls; }
+          ForallVarDecls(a, varDecls, p)(s);
+        }
+      } else {
+        if ForallVarDecls(a, varDecls, p)(s) == None {
+          NoneForallVarDecls(a, varDecls, p, s);
+          var vs :| (ValuesRespectDecls(a, vs, varDecls) && p(StateUpdVarDecls(s, varDecls, vs)) == None);
+
+          assert |vs| == |varDecls|;
+          var vs1 := vs[0..|varDecls1|];
+          var vs2 := vs[|varDecls1|..|varDecls|];
+
+          assert vs1+vs2 == vs;
+
+          assert varDecls1 == varDecls[0..|varDecls1|];
+          assert varDecls2 == varDecls[|varDecls1|..|varDecls|];
+
+          assert ValuesRespectDecls(a, vs1, varDecls1) by {
+            ValuesRespectDeclsSlice(a, vs, varDecls, 0, |varDecls1|);
+          }
+          assert ValuesRespectDecls(a, vs2, varDecls2) by {
+            ValuesRespectDeclsSlice(a, vs, varDecls, |varDecls1|, |varDecls|);
+          }
+
+          calc {
+            StateUpdVarDecls(s, varDecls1+varDecls2, vs1+vs2);
+            { StateUpdVarDeclsSplit2(s, varDecls1, varDecls2, vs1, vs2); }
+            StateUpdVarDecls(StateUpdVarDecls(s, varDecls1, vs1), varDecls2, vs2);
+          }
+
+          var s1 := StateUpdVarDecls(s, varDecls1, vs1);
+
+          assert ForallVarDecls(a, varDecls1, ForallVarDecls(a, varDecls2, p))(s) == None by {
+            assert ForallVarDecls(a, varDecls2, p)(s1) == None by {
+              assert p(StateUpdVarDecls(s1, varDecls2, vs2)) == None;
+              NoneForallVarDecls2(a, varDecls2, vs2, p, s1);
+            }
+            
+            NoneForallVarDecls2(a, varDecls1, vs1, ForallVarDecls(a, varDecls2, p), s);
+          }
+        } else if ForallVarDecls(a, varDecls, p)(s) == Some(true) {
+          assert ForallVarDecls(a, varDecls1, ForallVarDecls(a, varDecls2, p))(s) == Some(true) by {
+            forall vs1 | ValuesRespectDecls(a, vs1, varDecls1)
+            ensures ForallVarDecls(a, varDecls2, p)(StateUpdVarDecls(s, varDecls1, vs1)) == Some(true)
+            {
+              var s1 := StateUpdVarDecls(s, varDecls1, vs1);
+              forall vs2 | ValuesRespectDecls(a, vs2, varDecls2)
+              ensures p(StateUpdVarDecls(s1, varDecls2, vs2)) == Some(true)
+              {
+                var vs := vs1+vs2;
+                assert ValuesRespectDecls(a, vs, varDecls) by {
+                  ValuesRespectDeclsAppend(a, varDecls1, varDecls2, vs1, vs2);
+                }
+                calc {
+                  StateUpdVarDecls(s, varDecls1+varDecls2, vs1+vs2);
+                  { StateUpdVarDeclsSplit2(s, varDecls1, varDecls2, vs1, vs2); }
+                  StateUpdVarDecls(StateUpdVarDecls(s, varDecls1, vs1), varDecls2, vs2);
+                }
+                  
+                assert p(StateUpdVarDecls(s, varDecls, vs)) == Some(true) by {
+                  SomeTrueForallVarDecls2(a, varDecls, p, s, vs);
+                }
+              }
+              SomeTrueForallVarDecls(a, varDecls2, p, s1);
+            }
+            SomeTrueForallVarDecls(a, varDecls1, ForallVarDecls(a, varDecls2, p), s);
+          }
+        } else {
+          assert ForallVarDecls(a, varDecls, p)(s) == Some(false) by {
+            reveal ForallVarDecls();
+          }
+
+          forall vs1 | ValuesRespectDecls(a, vs1, varDecls1)
+          ensures ForallVarDecls(a, varDecls2, p)(StateUpdVarDecls(s, varDecls1, vs1)).Some?
+          {
+            var s1 := StateUpdVarDecls(s, varDecls1, vs1);
+            forall vs2 | ValuesRespectDecls(a, vs2, varDecls2)
+            ensures p(StateUpdVarDecls(s1, varDecls2, vs2)).Some?
+            {
+              var vs := vs1+vs2;
+              assert ValuesRespectDecls(a, vs, varDecls) by {
+                ValuesRespectDeclsAppend(a, varDecls1, varDecls2, vs1, vs2);
+              }
+              calc {
+                StateUpdVarDecls(s, varDecls1+varDecls2, vs1+vs2);
+                { StateUpdVarDeclsSplit2(s, varDecls1, varDecls2, vs1, vs2); }
+                StateUpdVarDecls(StateUpdVarDecls(s, varDecls1, vs1), varDecls2, vs2);
+              }
+                
+              assert p(StateUpdVarDecls(s, varDecls, vs)).Some? by {
+                SomeForallVarDecls2(a, varDecls, p, s, vs);
+              }
+            }
+            SomeForallVarDecls3(a, varDecls2, p, s1);
+          }
+
+          assert ForallVarDecls(a, varDecls1, ForallVarDecls(a, varDecls2, p))(s).Some? by {
+            SomeForallVarDecls3(a, varDecls1, ForallVarDecls(a, varDecls2, p), s);
+          }
+
+
+          SomeFalseForallVarDecls2(a, varDecls, p, s);
+
+          var vs :| ValuesRespectDecls(a, vs, varDecls) && p(StateUpdVarDecls(s, varDecls, vs)) == Some(false);
+
+          assert |vs| == |varDecls|;
+          var vs1 := vs[0..|varDecls1|];
+          var vs2 := vs[|varDecls1|..|varDecls|];
+
+          assert vs1+vs2 == vs;
+
+          assert varDecls1 == varDecls[0..|varDecls1|];
+          assert varDecls2 == varDecls[|varDecls1|..|varDecls|];
+
+          assert ValuesRespectDecls(a, vs1, varDecls1) by {
+            ValuesRespectDeclsSlice(a, vs, varDecls, 0, |varDecls1|);
+          }
+          assert ValuesRespectDecls(a, vs2, varDecls2) by {
+            ValuesRespectDeclsSlice(a, vs, varDecls, |varDecls1|, |varDecls|);
+          }
+          
+          calc {
+            StateUpdVarDecls(s, varDecls1+varDecls2, vs1+vs2);
+            { StateUpdVarDeclsSplit2(s, varDecls1, varDecls2, vs1, vs2); }
+            StateUpdVarDecls(StateUpdVarDecls(s, varDecls1, vs1), varDecls2, vs2);
+          }
+
+          var s1 := StateUpdVarDecls(s, varDecls1, vs1);
+
+          assert ForallVarDecls(a, varDecls2, p)(s1) == Some(false) by {
+            assert p(StateUpdVarDecls(s1, varDecls2, vs2)) == Some(false);
+            SomeFalseForallVarDecls(a, varDecls2, p, s1, vs2);
+          }
+
+          SomeFalseForallVarDecls(a, varDecls1, ForallVarDecls(a, varDecls2, p), s, vs1);
+        }
+      }
+    }
+}
